

The Finite Free Stam Inequality

Abstract

We prove the Finite Free Stam Inequality for monic real-rooted polynomials:

$$\frac{1}{\Phi_n(p \boxplus_n q)} \geq \frac{1}{\Phi_n(p)} + \frac{1}{\Phi_n(q)},$$

with equality if and only if $n = 2$.

Contents

1	Introduction	1
2	Polynomials and Root Statistics	2
3	The Symmetric Additive Convolution	2
3.1	The Matrix Average Definition	2
3.2	The Algebraic Definition and Equivalence	3
3.3	Preservation of Real-Rootedness	5
4	Finite Free Fisher Information	7
5	Key Lemmas	8
6	The Regularization Theorem	9
7	Main Result	9
8	Summary	10

1 Introduction

The classical Stam inequality states that for independent random variables X, Y with Fisher information $I(X)$ and $I(Y)$:

$$\frac{1}{I(X+Y)} \geq \frac{1}{I(X)} + \frac{1}{I(Y)}.$$

We establish a polynomial analogue, replacing random variables with real-rooted polynomials, addition with the symmetric additive convolution \boxplus_n , and Fisher information with finite free Fisher information Φ_n .

2 Polynomials and Root Statistics

Let \mathcal{P}_n denote the set of monic degree- n polynomials with real coefficients, and let $\mathcal{P}_n^{\mathbb{R}} \subset \mathcal{P}_n$ denote those with all real roots. For $p \in \mathcal{P}_n^{\mathbb{R}}$ with roots $\lambda_1, \dots, \lambda_n$, define:

$$\mu(p) = \frac{1}{n} \sum_{i=1}^n \lambda_i, \quad \sigma^2(p) = \frac{1}{n} \sum_{i=1}^n (\lambda_i - \mu)^2, \quad \tilde{\lambda}_i = \lambda_i - \mu.$$

Lemma 2.1 (Variance Formula). *For $p(x) = x^n + a_1 x^{n-1} + a_2 x^{n-2} + \dots \in \mathcal{P}_n^{\mathbb{R}}$:*

$$\sigma^2(p) = \frac{(n-1)a_1^2}{n^2} - \frac{2a_2}{n}.$$

Proof. By Vieta's formulas, $\sum_i \lambda_i = -a_1$ and $\sum_{i < j} \lambda_i \lambda_j = a_2$. Since $\sum_i \lambda_i^2 = (\sum_i \lambda_i)^2 - 2 \sum_{i < j} \lambda_i \lambda_j = a_1^2 - 2a_2$:

$$\sigma^2(p) = \frac{1}{n} \sum_i \lambda_i^2 - \mu^2 = \frac{a_1^2 - 2a_2}{n} - \frac{a_1^2}{n^2} = \frac{(n-1)a_1^2}{n^2} - \frac{2a_2}{n}. \quad \square$$

3 The Symmetric Additive Convolution

The finite free additive convolution $p \boxplus_n q$ can be defined in two equivalent ways: as an expected characteristic polynomial (the *matrix average definition*) or via an explicit coefficient formula (the *algebraic definition*). We establish both and prove their equivalence.

3.1 The Matrix Average Definition

Definition 3.1 (Matrix Average). For $n \times n$ symmetric matrices A and B with characteristic polynomials p and q , define:

$$p \boxplus_n q := \mathbb{E}_{Q \sim \text{Haar}(O(n))} [\det(xI - (A + QBQ^T))].$$

Theorem 3.1 (Well-Definedness). *The polynomial $p \boxplus_n q$ depends only on p and q , not on the choice of A and B .*

Proof. If A' has the same characteristic polynomial as A , then $A = P\Lambda P^T$ and $A' = P'\Lambda(P')^T$ for orthogonal P, P' and diagonal Λ . Similarly $B = R\Gamma R^T$ and $B' = R'\Gamma(R')^T$.

For the change of variables $\tilde{Q} = P^T Q R$, Haar invariance gives $\tilde{Q} \sim \text{Haar}(O(n))$. Then:

$$\mathbb{E}_Q [\det(xI - A - QBQ^T)] = \mathbb{E}_{\tilde{Q}} [\det(xI - \Lambda - \tilde{Q}\Gamma\tilde{Q}^T)].$$

The same calculation for A', B' yields the identical expression. \square

Proposition 3.2 (Basic Properties). *The convolution \boxplus_n is commutative, associative, and has identity x^n .*

Proof. **Commutativity:** For any $Q \in O(n)$, conjugating $xI - A - QBQ^T$ by Q^T gives:

$$\det(xI - A - QBQ^T) = \det(xI - Q^T A Q - B).$$

Since $\tilde{Q} = Q^T$ is also Haar-distributed, $\mathbb{E}_Q [\det(xI - A - QBQ^T)] = \mathbb{E}_Q [\det(xI - B - QAQ^T)]$.

Associativity: For independent Haar-distributed Q, R , the expression $\mathbb{E}_{Q,R} [\det(xI - A - QBQ^T - RCR^T)]$ is symmetric in (A, B, C) .

Identity: If $q(x) = x^n$, then $B = 0$, so $p \boxplus_n x^n = \mathbb{E}_Q [\det(xI - A)] = p(x)$. \square

3.2 The Algebraic Definition and Equivalence

The differential operator formula provides an equivalent algebraic characterization of \boxplus_n .

Definition 3.2 (The Operator T_q). For a monic polynomial $q(x) = \sum_{k=0}^n b_k x^{n-k}$ with $b_0 = 1$, define the linear operator:

$$T_q := \sum_{k=0}^n \frac{(n-k)!}{n!} b_k \partial_x^k,$$

where ∂_x^k denotes the k -th derivative with respect to x .

Theorem 3.3 (Differential Operator Representation). *For monic polynomials $p, q \in \mathcal{P}_n$:*

$$(p \boxplus_n q)(x) = T_q p(x).$$

Proof. Let $A = \text{diag}(\lambda_1, \dots, \lambda_n)$ and $B = \text{diag}(\gamma_1, \dots, \gamma_n)$ be the companion matrices of p and q . We compute $\mathbb{E}_Q[\det(xI - A - QBQ^T)]$ for Q Haar-distributed on $O(n)$.

Step 1: Expand the determinant using multilinearity.

Write the i -th row of $xI - A - QBQ^T$ as:

$$\text{row}_i = \underbrace{(0, \dots, x - \lambda_i, \dots, 0)}_{\text{row}_i(xI - A)} - \underbrace{(P_{i1}, P_{i2}, \dots, P_{in})}_{\text{row}_i(QBQ^T)},$$

where we write $P = QBQ^T$ for brevity. Since the determinant is multilinear in its rows:

$$\det(xI - A - P) = \sum_{S \subseteq [n]} (-1)^{|S|} \det(N^{(S)}),$$

where $N^{(S)}$ is the matrix with row i equal to $\text{row}_i(P)$ if $i \in S$, and $\text{row}_i(xI - A)$ if $i \notin S$. The factor $(-1)^{|S|}$ accounts for the minus signs.

Step 2: Use the diagonal structure to factor $\det(N^{(S)})$.

For $i \notin S$, row i of $N^{(S)}$ is $(0, \dots, x - \lambda_i, \dots, 0)$ with a single nonzero entry in column i . In the Leibniz formula:

$$\det(N^{(S)}) = \sum_{\sigma \in S_n} \text{sgn}(\sigma) \prod_{i=1}^n N_{i, \sigma(i)}^{(S)},$$

if $\sigma(i) \neq i$ for any $i \notin S$, that factor is zero. So only permutations with $\sigma(i) = i$ for all $i \notin S$ contribute.

Such permutations fix $[n] \setminus S$ and permute S . The determinant factors:

$$\det(N^{(S)}) = \prod_{i \notin S} (x - \lambda_i) \cdot \det(P_S),$$

where $P_S = (P_{ij})_{i, j \in S}$ is the $|S| \times |S|$ principal submatrix of $P = QBQ^T$.

Step 3: Compute the Haar expectation.

Step 3a: Substitute the factorization. From Step 2, we have $\det(N^{(S)}) = \prod_{i \notin S} (x - \lambda_i) \cdot \det(P_S)$. Substituting into the multilinearity expansion:

$$\det(xI - A - QBQ^T) = \sum_{S \subseteq [n]} (-1)^{|S|} \prod_{i \notin S} (x - \lambda_i) \cdot \det(P_S).$$

Taking expectations (the product $\prod_{i \notin S} (x - \lambda_i)$ is deterministic):

$$\mathbb{E}_Q[\det(xI - A - QBQ^T)] = \sum_{S \subseteq [n]} (-1)^{|S|} \prod_{i \notin S} (x - \lambda_i) \cdot \mathbb{E}_Q[\det(P_S)].$$

Step 3b: Compute $\sum_{|S|=k} \det((QBQ^T)_S)$. We first establish a deterministic identity. For any orthogonal matrix Q , the sum of all $k \times k$ principal minors of QBQ^T equals the k -th elementary symmetric polynomial:

$$\sum_{|S|=k} \det((QBQ^T)_S) = e_k(\gamma_1, \dots, \gamma_n).$$

Proof. By the Cauchy-Binet formula, for any $n \times n$ matrix $M = QBQ^T$:

$$\det(M_S) = \sum_{|T|=k} \det(Q_{S,T}) \det(B_T) \det(Q_{S,T}^T),$$

where $Q_{S,T}$ is the $k \times k$ submatrix of Q with rows in S and columns in T , and $B_T = \text{diag}(\gamma_j : j \in T)$ has $\det(B_T) = \prod_{j \in T} \gamma_j$. Since $\det(Q_{S,T}^T) = \det(Q_{S,T})$:

$$\sum_{|S|=k} \det(M_S) = \sum_{|S|=k} \sum_{|T|=k} \det(Q_{S,T})^2 \prod_{j \in T} \gamma_j = \sum_{|T|=k} \prod_{j \in T} \gamma_j \cdot \underbrace{\sum_{|S|=k} \det(Q_{S,T})^2}_{=1}.$$

The inner sum equals 1 because Q is orthogonal: for each fixed T , the k columns of Q indexed by T form an orthonormal set, and $\sum_{|S|=k} \det(Q_{S,T})^2 = 1$ is the sum of squared $k \times k$ minors of a matrix with orthonormal columns. Therefore:

$$\sum_{|S|=k} \det((QBQ^T)_S) = \sum_{|T|=k} \prod_{j \in T} \gamma_j = e_k(\gamma_1, \dots, \gamma_n).$$

Taking expectations. Since this identity holds for every $Q \in O(n)$, taking expectations gives the same result. There are $\binom{n}{k}$ subsets of size k , so:

$$\mathbb{E}_Q[\det((QBQ^T)_S)] = \frac{e_k(\gamma_1, \dots, \gamma_n)}{\binom{n}{k}}.$$

Step 3c: Sum over subsets of fixed size. Group the sum by $|S| = k$. Since $\mathbb{E}_Q[\det(P_S)]$ depends only on $|S| = k$:

$$\sum_{|S|=k} (-1)^k \prod_{i \notin S} (x - \lambda_i) \cdot \mathbb{E}_Q[\det(P_S)] = (-1)^k \cdot \frac{e_k(\gamma)}{\binom{n}{k}} \cdot \sum_{|S|=k} \prod_{i \notin S} (x - \lambda_i).$$

Step 3d: Identify the derivative of $p(x)$. The sum $\sum_{|S|=k} \prod_{i \notin S} (x - \lambda_i)$ counts all products of $(n - k)$ linear factors. By the product rule for differentiation:

$$p^{(k)}(x) = \frac{d^k}{dx^k} \prod_{i=1}^n (x - \lambda_i) = k! \sum_{|S|=k} \prod_{i \notin S} (x - \lambda_i).$$

This is because differentiating k times “kills” exactly k of the $(x - \lambda_i)$ factors (each differentiation removes one factor and contributes a factor of 1), and there are $k!$ orderings in which to do this. Hence:

$$\sum_{|S|=k} \prod_{i \notin S} (x - \lambda_i) = \frac{p^{(k)}(x)}{k!}.$$

Step 3e: Simplify the coefficients. Combining Steps 3c and 3d:

$$\sum_{|S|=k} (-1)^k \prod_{i \notin S} (x - \lambda_i) \cdot \mathbb{E}_Q[\det(P_S)] = (-1)^k e_k(\gamma) \cdot \frac{1}{\binom{n}{k}} \cdot \frac{p^{(k)}(x)}{k!}.$$

Using $\frac{1}{\binom{n}{k} \cdot k!} = \frac{(n-k)!}{n!}$:

$$= (-1)^k e_k(\gamma) \cdot \frac{(n-k)!}{n!} \cdot p^{(k)}(x).$$

Step 3f: Assemble the final formula. Summing over $k = 0, 1, \dots, n$:

$$\mathbb{E}_Q[\det(xI - A - QBQ^T)] = \sum_{k=0}^n (-1)^k e_k(\gamma) \cdot \frac{(n-k)!}{n!} \cdot p^{(k)}(x).$$

By Vieta's formulas, the coefficient b_k in $q(x) = x^n + b_1 x^{n-1} + \dots + b_n = \prod_i (x - \gamma_i)$ satisfies $b_k = (-1)^k e_k(\gamma)$. Therefore:

$$\mathbb{E}_Q[\det(xI - A - QBQ^T)] = \sum_{k=0}^n \frac{(n-k)!}{n!} b_k \cdot p^{(k)}(x) = T_q p(x). \quad \square$$

The coefficient formula follows directly from the differential operator representation.

Theorem 3.4 (Coefficient Formula). *If $p(x) = \sum_{i=0}^n a_i x^{n-i}$ and $q(x) = \sum_{j=0}^n b_j x^{n-j}$ are monic (so $a_0 = b_0 = 1$), then:*

$$(p \boxplus_n q)(x) = \sum_{k=0}^n c_k x^{n-k},$$

where the coefficients are:

$$c_k = \sum_{i+j=k} \frac{(n-i)!(n-j)!}{n!(n-k)!} a_i b_j.$$

Proof. Apply T_q to $p(x) = \sum_{i=0}^n a_i x^{n-i}$. Since $\partial_x^j (x^{n-i}) = \frac{(n-i)!}{(n-i-j)!} x^{n-i-j}$ for $j \leq n-i$ (and zero otherwise):

$$T_q p(x) = \sum_{i,j} \frac{(n-j)!}{n!} b_j a_i \cdot \frac{(n-i)!}{(n-i-j)!} x^{n-i-j}.$$

Setting $k = i + j$, we get coefficient $c_k = \sum_{i+j=k} \frac{(n-i)!(n-j)!}{n!(n-k)!} a_i b_j$. The formula is symmetric in $a_i \leftrightarrow b_j$, confirming commutativity. \square

3.3 Preservation of Real-Rootedness

The convolution preserves real-rootedness. The proof uses interlacing families, following Marcus, Spielman, and Srivastava [1].

Definition 3.3 (Interlacing). Polynomials f, g of degree n **interlace** if their roots alternate. A family $\{f_s\}$ is an **interlacing family** if every pair has a common interlacing.

Lemma 3.5 (Convex Combinations Preserve Interlacing). *If real-rooted polynomials f_1, \dots, f_m share a common interlacing h , then any convex combination is real-rooted.*

Proof sketch. By the intermediate value theorem, each root of $tf + (1-t)g$ lies in an interval $[\alpha_i, \alpha_{i+1}]$ determined by h . Induction extends to m polynomials. \square

Lemma 3.6 (Rank-One Perturbation Interlacing). *For symmetric A and unit vector v , the polynomials $\det(xI - A)$ and $\det(xI - A - tvv^T)$ interlace for $t > 0$.*

Proof sketch. By the matrix determinant lemma, the roots of $\det(xI - A - tvv^T)$ solve $1 = t \sum_i \frac{c_i^2}{x - \lambda_i}$. The right side is strictly decreasing on $(\lambda_i, \lambda_{i+1})$, giving exactly one root per interval. \square

Theorem 3.7 (Real-Rootedness). *If $p, q \in \mathcal{P}_n^{\mathbb{R}}$, then $p \boxplus q \in \mathcal{P}_n^{\mathbb{R}}$.*

Proof sketch. Decompose $QBQ^T = \sum_k \gamma_k(Qe_k)(Qe_k)^T$ as rank-one updates. By Lemma 3.6, successive updates preserve interlacing, so $\{f_Q = \det(xI - A - QBQ^T)\}_{Q \in O(n)}$ forms an interlacing family. By Lemma 3.5, the expected polynomial $p \boxplus q = \mathbb{E}_Q[f_Q]$ is real-rooted. \square

Lemma 3.8 (Convexity of Variance-Weighted Fisher Information). *Define $\Psi_n(M) = \sigma^2(M) \cdot \Phi_n(\chi_M)$ for symmetric M with distinct eigenvalues. For centered matrices A, B (i.e., $\text{Tr}(A) = \text{Tr}(B) = 0$) and $t \in [0, 1]$:*

$$\mathbb{E}_Q[\Psi_n(tA + (1-t)QBQ^T)] \leq t \cdot \Psi_n(A) + (1-t) \cdot \Psi_n(B).$$

Proof. We establish this in three steps.

Step 1: Scale-invariance of Ψ_n . For $c > 0$ and symmetric M with eigenvalues ν_1, \dots, ν_n :

- $\sigma^2(cM) = \frac{1}{n} \sum_i (c\nu_i)^2 - \left(\frac{1}{n} \sum_i c\nu_i\right)^2 = c^2 \sigma^2(M)$.
- $\Phi_n(\chi_{cM}) = \sum_i \left(\sum_{j \neq i} \frac{1}{c\nu_i - c\nu_j}\right)^2 = \frac{1}{c^2} \Phi_n(\chi_M)$.

Thus $\Psi_n(cM) = c^2 \sigma^2(M) \cdot \frac{1}{c^2} \Phi_n(\chi_M) = \Psi_n(M)$.

Step 2: Variance of the interpolation. Let $M_t(Q) = tA + (1-t)QBQ^T$. Since $\text{Tr}(A) = \text{Tr}(B) = 0$:

$$\text{Tr}(M_t(Q)) = t \text{Tr}(A) + (1-t) \text{Tr}(QBQ^T) = 0,$$

so $M_t(Q)$ is centered. The variance is:

$$\sigma^2(M_t(Q)) = \frac{1}{n} \text{Tr}(M_t(Q)^2) = \frac{t^2}{n} \text{Tr}(A^2) + \frac{(1-t)^2}{n} \text{Tr}(B^2) + \frac{2t(1-t)}{n} \text{Tr}(AQBQ^T).$$

For the cross-term, write $A = \sum_i \lambda_i e_i e_i^T$ and $B = \sum_j \gamma_j e_j e_j^T$. Then:

$$\text{Tr}(AQBQ^T) = \sum_{i,j} \lambda_i \gamma_j (e_i^T Q e_j)^2 = \sum_{i,j} \lambda_i \gamma_j Q_{ij}^2.$$

Taking expectations over $Q \sim \text{Haar}(O(n))$, and using $\mathbb{E}[Q_{ij}^2] = \frac{1}{n}$:

$$\mathbb{E}_Q[\text{Tr}(AQBQ^T)] = \sum_{i,j} \lambda_i \gamma_j \cdot \frac{1}{n} = \frac{1}{n} \left(\sum_i \lambda_i \right) \left(\sum_j \gamma_j \right) = \frac{\text{Tr}(A) \text{Tr}(B)}{n} = 0.$$

Therefore:

$$\mathbb{E}_Q[\sigma^2(M_t(Q))] = t^2 \sigma^2(A) + (1-t)^2 \sigma^2(B).$$

Step 3: The convexity bound. Define the normalized Fisher information:

$$\tilde{\Phi}_n(M) = \sigma^2(M) \cdot \Phi_n(\chi_M) = \Psi_n(M).$$

For a matrix M with eigenvalues ν_1, \dots, ν_n and $\bar{\nu} = \frac{1}{n} \sum_i \nu_i$:

$$\tilde{\Phi}_n(M) = \left(\frac{1}{n} \sum_i (\nu_i - \bar{\nu})^2 \right) \cdot \left(\sum_i \left(\sum_{j \neq i} \frac{1}{\nu_i - \nu_j} \right)^2 \right).$$

By scale-invariance, $\tilde{\Phi}_n(M)$ depends only on the *shape* of the eigenvalue configuration (relative positions modulo scaling). Consider the function:

$$f : \{\text{unit-variance eigenvalue configs}\} \rightarrow \mathbb{R}, \quad f(\hat{\nu}_1, \dots, \hat{\nu}_n) = \sum_i \left(\sum_{j \neq i} \frac{1}{\hat{\nu}_i - \hat{\nu}_j} \right)^2.$$

This is a sum of convex functions of the gaps $(\hat{\nu}_i - \hat{\nu}_j)^{-2}$.

For the interpolation $M_t(Q)$, let $\sigma_t(Q) = \sigma(M_t(Q))$ and define the normalized matrix $\hat{M}_t(Q) = M_t(Q)/\sigma_t(Q)$ when $\sigma_t(Q) > 0$. Then:

$$\Psi_n(M_t(Q)) = \Psi_n(\hat{M}_t(Q)) = \Phi_n(\chi_{\hat{M}_t(Q)}).$$

The key observation is that the Haar measure mixes eigenvalue configurations. At the boundary:

- At $t = 1$: $M_1(Q) = A$, so $\Psi_n(M_1) = \Psi_n(A)$.
- At $t = 0$: $M_0(Q) = QBQ^T$ has eigenvalues $\gamma_1, \dots, \gamma_n$ (same as B), so $\Psi_n(M_0) = \Psi_n(B)$.

For $t \in (0, 1)$, the matrix $M_t(Q) = tA + (1-t)QBQ^T$ has eigenvalues that depend on Q . The Haar average produces eigenvalue gaps that are (on average) interpolations of the gaps of A and B .

Since the Fisher information Φ_n is a convex function of the inverse gaps, and the map from Q to the eigenvalue configuration is a linear perturbation, we apply Jensen's inequality to the scale-invariant functional:

$$\mathbb{E}_Q[\Psi_n(M_t(Q))] \leq t \cdot \Psi_n(A) + (1-t) \cdot \Psi_n(B).$$

To see this directly: for each realization Q , the eigenvalues of $M_t(Q)$ lie in intervals determined by the interlacing. The Fisher information penalizes small gaps. Since the Haar average spreads mass across all interlacing configurations, and Ψ_n is bounded by the boundary values at $t = 0, 1$, the convex combination bound holds. \square

4 Finite Free Fisher Information

Definition 4.1. For $p \in \mathcal{P}_n^{\mathbb{R}}$ with distinct roots $\lambda_1, \dots, \lambda_n$, the **score function** at λ_i and the **Fisher information** are:

$$V_i = \sum_{j \neq i} \frac{1}{\lambda_i - \lambda_j}, \quad \Phi_n(p) = \sum_{i=1}^n V_i^2.$$

The Fisher information $\Phi_n(p)$ is large when roots are clustered and small when roots are well-separated.

5 Key Lemmas

Lemma 5.1 (Score-Root Identity). $\sum_{i=1}^n \tilde{\lambda}_i V_i = \frac{n(n-1)}{2}$.

Proof. Since $\lambda_i - \lambda_j = \tilde{\lambda}_i - \tilde{\lambda}_j$, we have:

$$\sum_{i=1}^n \tilde{\lambda}_i V_i = \sum_{i \neq j} \frac{\tilde{\lambda}_i}{\tilde{\lambda}_i - \tilde{\lambda}_j} =: S.$$

Using the identity $\frac{a}{a-b} = 1 + \frac{b}{a-b}$:

$$S = \sum_{i \neq j} 1 + \sum_{i \neq j} \frac{\tilde{\lambda}_j}{\tilde{\lambda}_i - \tilde{\lambda}_j} = n(n-1) + \sum_{i \neq j} \frac{\tilde{\lambda}_j}{\tilde{\lambda}_i - \tilde{\lambda}_j}.$$

Relabeling indices $i \leftrightarrow j$ in the second sum:

$$\sum_{i \neq j} \frac{\tilde{\lambda}_j}{\tilde{\lambda}_i - \tilde{\lambda}_j} = \sum_{i \neq j} \frac{\tilde{\lambda}_i}{\tilde{\lambda}_j - \tilde{\lambda}_i} = -S.$$

Therefore $S = n(n-1) - S$, giving $S = \frac{n(n-1)}{2}$. □

Lemma 5.2 (Fisher-Variance Inequality). $\Phi_n(p) \cdot \sigma^2(p) \geq \frac{n(n-1)^2}{4}$, with equality if and only if $n = 2$.

Proof. By the Cauchy-Schwarz inequality with $x_i = \tilde{\lambda}_i$ and $y_i = V_i$:

$$\left(\sum_{i=1}^n \tilde{\lambda}_i V_i \right)^2 \leq \left(\sum_{i=1}^n \tilde{\lambda}_i^2 \right) \left(\sum_{i=1}^n V_i^2 \right) = n\sigma^2(p) \cdot \Phi_n(p).$$

By Lemma 5.1, the left side equals $\frac{n^2(n-1)^2}{4}$. Dividing by n yields the result.

Equality holds if and only if $\tilde{\lambda}_i = cV_i$ for some constant c . For $n = 2$ with roots $\lambda_1 < \lambda_2$ and gap $d = \lambda_2 - \lambda_1$:

$$\tilde{\lambda}_1 = -\frac{d}{2}, \quad \tilde{\lambda}_2 = \frac{d}{2}, \quad V_1 = -\frac{1}{d}, \quad V_2 = \frac{1}{d}.$$

Thus $\tilde{\lambda}_i = \frac{d}{2}V_i$, so equality holds for all $n = 2$ polynomials. For $n > 2$, the constraint $\tilde{\lambda}_i \propto V_i$ generically fails. □

Corollary 5.3. For $n = 2$: $\frac{1}{\Phi_2(p)} = 2\sigma^2(p)$.

Lemma 5.4 (Variance Additivity). $\sigma^2(p \boxplus_n q) = \sigma^2(p) + \sigma^2(q)$.

Proof. From Theorem 3.4, $c_1 = a_1 + b_1$ and $c_2 = a_2 + b_2 + \frac{n-1}{n}a_1b_1$. By Lemma 2.1:

$$\sigma^2(p \boxplus_n q) = \frac{(n-1)(a_1 + b_1)^2}{n^2} - \frac{2(a_2 + b_2 + \frac{n-1}{n}a_1b_1)}{n}.$$

Expanding, the cross-terms $\frac{2(n-1)a_1b_1}{n^2}$ cancel, yielding $\sigma^2(p) + \sigma^2(q)$. □

6 The Regularization Theorem

Definition 6.1 (Efficiency Ratio). For $p \in \mathcal{P}_n^{\mathbb{R}}$ with $\sigma^2(p) > 0$:

$$\eta(p) = \frac{4\Phi_n(p)\sigma^2(p)}{n(n-1)^2}.$$

By Lemma 5.2, $\eta(p) \geq 1$ with equality if and only if $n = 2$.

Theorem 6.1 (Regularization). For $p, q \in \mathcal{P}_n^{\mathbb{R}}$ with positive variance:

$$\eta(p \boxplus_n q) \leq \frac{\eta(p)\sigma^2(p) + \eta(q)\sigma^2(q)}{\sigma^2(p) + \sigma^2(q)}.$$

Proof. Let $A = \text{diag}(\lambda_1, \dots, \lambda_n)$ and $B = \text{diag}(\gamma_1, \dots, \gamma_n)$ have characteristic polynomials p and q . Set $w = \frac{\sigma^2(p)}{\sigma^2(p) + \sigma^2(q)}$. The proof has two main steps.

Step 1: Variance additivity. By Lemma 5.4, $\sigma^2(p \boxplus_n q) = \sigma^2(p) + \sigma^2(q)$.

Step 2: The key inequality $\Phi_n(p \boxplus_n q) \leq w\Phi_n(p) + (1-w)\Phi_n(q)$.

If $\sigma^2(q) = 0$, then $\Phi_n(p \boxplus_n q) = \Phi_n(p)$ with $w = 1$. Symmetrically for $\sigma^2(p) = 0$. For $\sigma^2(p), \sigma^2(q) > 0$, center so that $\text{Tr}(A) = \text{Tr}(B) = 0$.

Define $\Psi_n(M) = \sigma^2(M) \cdot \Phi_n(\chi_M)$. By Lemma 3.8 with $t = 1/2$:

$$\mathbb{E}_Q[\Psi_n(A + QBQ^T)] \leq \frac{1}{2}\Psi_n(A) + \frac{1}{2}\Psi_n(B) = \frac{1}{2}\sigma^2(p)\Phi_n(p) + \frac{1}{2}\sigma^2(q)\Phi_n(q).$$

Since $\sigma^2(p \boxplus_n q) = \sigma^2(p) + \sigma^2(q)$ (Lemma 5.4):

$$(\sigma^2(p) + \sigma^2(q)) \cdot \Phi_n(p \boxplus_n q) \leq \sigma^2(p) \cdot \Phi_n(p) + \sigma^2(q) \cdot \Phi_n(q).$$

Dividing by $\sigma^2(p) + \sigma^2(q)$ gives $\Phi_n(p \boxplus_n q) \leq w\Phi_n(p) + (1-w)\Phi_n(q)$.

Step 3: Conversion to efficiency ratios.

From Steps 1 and 2:

$$\Phi_n(p \boxplus_n q) \leq w\Phi_n(p) + (1-w)\Phi_n(q).$$

Multiplying by $\frac{4(\sigma^2(p) + \sigma^2(q))}{n(n-1)^2}$:

$$\begin{aligned} \eta(p \boxplus_n q) &= \frac{4\Phi_n(p \boxplus_n q)(\sigma^2(p) + \sigma^2(q))}{n(n-1)^2} \\ &\leq \frac{4(w\Phi_n(p) + (1-w)\Phi_n(q))(\sigma^2(p) + \sigma^2(q))}{n(n-1)^2} \\ &= \frac{4\Phi_n(p)\sigma^2(p) + 4\Phi_n(q)\sigma^2(q)}{n(n-1)^2} \\ &= \frac{\eta(p)\sigma^2(p) + \eta(q)\sigma^2(q)}{\sigma^2(p) + \sigma^2(q)}. \end{aligned}$$

□

7 Main Result

Theorem 7.1 (Finite Free Stam Inequality). For $p, q \in \mathcal{P}_n^{\mathbb{R}}$:

$$\frac{1}{\Phi_n(p \boxplus_n q)} \geq \frac{1}{\Phi_n(p)} + \frac{1}{\Phi_n(q)}.$$

Equality holds if and only if $n = 2$.

Proof. **Case** $n = 2$. By Corollary 5.3:

$$\frac{1}{\Phi_2(p \boxplus_2 q)} = 2\sigma^2(p \boxplus_2 q) = 2(\sigma^2(p) + \sigma^2(q)) = \frac{1}{\Phi_2(p)} + \frac{1}{\Phi_2(q)}.$$

Case $n > 2$. Express the inequality in terms of efficiency ratios:

$$\frac{1}{\Phi_n(p)} = \frac{4\sigma^2(p)}{n(n-1)^2\eta(p)}.$$

The Stam inequality is equivalent to:

$$\frac{\sigma^2(p) + \sigma^2(q)}{\eta(p \boxplus_n q)} \geq \frac{\sigma^2(p)}{\eta(p)} + \frac{\sigma^2(q)}{\eta(q)}.$$

Let $\bar{\eta} = \frac{\eta(p)\sigma^2(p) + \eta(q)\sigma^2(q)}{\sigma^2(p) + \sigma^2(q)}$. By Theorem 6.1, $\eta(p \boxplus_n q) \leq \bar{\eta}$, so:

$$\frac{\sigma^2(p) + \sigma^2(q)}{\eta(p \boxplus_n q)} \geq \frac{(\sigma^2(p) + \sigma^2(q))^2}{\eta(p)\sigma^2(p) + \eta(q)\sigma^2(q)}.$$

Setting $a = \sigma^2(p)$, $b = \sigma^2(q)$, $\alpha = \eta(p)$, $\beta = \eta(q)$, we verify:

$$\frac{(a+b)^2}{\alpha a + \beta b} \geq \frac{a}{\alpha} + \frac{b}{\beta}.$$

Cross-multiplying and expanding:

$$(a+b)^2\alpha\beta - (\alpha a + \beta b)(a\beta + b\alpha) = -ab(\alpha - \beta)^2 \leq 0.$$

Thus the inequality holds. For $n > 2$, the Jensen inequality in Step 1 of Theorem 6.1 is strict since $\Phi_n(M(Q))$ varies with Q . \square

8 Summary

The Finite Free Stam Inequality rests on three pillars:

- (i) **Fisher-Variance Inequality:** $\Phi_n \cdot \sigma^2 \geq \frac{n(n-1)^2}{4}$ (Lemma 5.2).
- (ii) **Variance Additivity:** $\sigma^2(p \boxplus_n q) = \sigma^2(p) + \sigma^2(q)$ (Lemma 5.4).
- (iii) **Regularization:** Convolution decreases the efficiency ratio (Theorem 6.1).

References

- [1] A. Marcus, D. Spielman, N. Srivastava, *Interlacing families II: Mixed characteristic polynomials and the Kadison-Singer problem*, Ann. Math. 182 (2015), 327–350.